Combining Trace and Program into a single entity, and forcing a decode function on Encodings

HMem/Computability/TracedProgram.lean
@@ -13,8 +13,19 @@ inductive TracedProgram {α: Type _} [Complexity.Encoding α Memory] {β: Type _
 | recurse (dst src: Source) (next: TracedProgram f)
 
 namespace TracedProgram
-
 variable {α: Type _} [Complexity.Encoding α Memory] {β: Type _} [Complexity.Encoding β Memory] {f: α → β}
+
+@[simp] def build: List (TracedProgram f → TracedProgram f) → TracedProgram f
+| [] => .exit
+| p::ps => p (build ps)
+
+@[simp] def setv (dst: Source) (b: Bool): TracedProgram f → TracedProgram f := op (.vop (λ _ ↦ b) dst finZeroElim)
+@[simp] def setm (dst: Source) (src: Memory): TracedProgram f  → TracedProgram f := op (.const dst src)
+@[simp] def copyv (dst src: Source): TracedProgram f  → TracedProgram f := op (.vop (λ f ↦ f 0) dst (λ (_: Fin 1) ↦ src))
+@[simp] def copy (dst src: Source): TracedProgram f  → TracedProgram f := op (.mop .COPY dst src)
+@[simp] def move (dst src: Source): TracedProgram f  → TracedProgram f := op (.mop .MOVE dst src)
+@[simp] def swap (dst src: Source): TracedProgram f  → TracedProgram f := op (.mop .SWAP dst src)
+@[simp] def ifv (src: Source) (pos: List (TracedProgram f  → TracedProgram f)) (neg: List (TracedProgram f  → TracedProgram f)): TracedProgram f := branch (.ifTrue (λ f ↦ f 0) (λ (_: Fin 1) ↦ src)) (build pos) (build neg)
 
 @[match_pattern] def subroutine' (dst src: Source) {γ: Type _} (_hγ: Complexity.Encoding γ Memory) {δ: Type _} (_hδ: Complexity.Encoding δ Memory)
     (func: γ → δ) (_h: Computable Encoding.Model func) (next: TracedProgram f): TracedProgram f :=
@@ -32,60 +43,160 @@ inductive Step (α: Type _) [Complexity.Encoding α Memory]
 | op (inst: OpInstruction)
 | branch (inst: BranchInstruction)
 | subroutine (dst src: Source) {γ: Type _} [Complexity.Encoding γ Memory] {δ: Type _} [Complexity.Encoding δ Memory]
-  (func: γ → δ) [Computable Encoding.Model func] (γ: arg)
+  (func: γ → δ) [Computable Encoding.Model func] (arg: γ)
 | recurse (dst src: Source) (arg: α)
 
-def foldlInternal {θ: Type _} (tp: TracedProgram f) (m: Memory) (g: θ → Step α → Memory → θ) (acc: θ): Option θ :=
+def foldrInternal {θ: Type _} (tp: TracedProgram f) (m: Memory) (acc: θ) (g: Step α → Memory → θ → θ): Option θ :=
   match tp with
-  | exit => some (g acc .exit m)
-  | op inst next => next.foldlInternal (inst.apply m) g (g acc (.op inst) m)
-  | branch inst pos neg => match inst.apply m with
-    | true => pos.foldlInternal m g (g acc (.branch inst) m)
-    | false => neg.foldlInternal m g (g acc (.branch inst) m)
+  | exit => some (g .exit m acc)
+  | op inst next => (next.foldrInternal (inst.apply m) acc g).map (g (.op inst) m)
+  | branch inst pos neg =>
+    if (inst.apply m)
+    then ((pos.foldrInternal m acc g).map (g (.branch inst) m))
+    else ((neg.foldrInternal m acc g).map (g (.branch inst) m))
   | subroutine' dst src _ _ func _ next =>
     (Complexity.decode _ (m.getms src)).bind
-    (λ arg ↦ next.foldlInternal (m.setms dst (Complexity.encode (func arg))) g (g acc (.subroutine dst src func arg) m))
+    (λ arg ↦ ((next.foldrInternal (m.setms dst (Complexity.encode (func arg))) acc g).map (g (.subroutine dst src func arg) m)))
   | recurse dst src next =>
     (Complexity.decode _ (m.getms src)).bind
-    (λ arg ↦ next.foldlInternal (m.setms dst (Complexity.encode (f arg))) g (g acc (.recurse dst src arg) m))
+    (λ arg ↦ (next.foldrInternal (m.setms dst (Complexity.encode (f arg))) acc g).map (g (.recurse dst src arg) m))
 
-def foldl (tp: TracedProgram f) (a: α): (θ → Step α → Memory → θ) → θ → Option θ :=
-  foldlInternal tp (Complexity.encode a)
+@[simp] def foldr (tp: TracedProgram f) (a: α): θ → (Step α → Memory → θ → θ) → Option θ :=
+  foldrInternal tp (Complexity.encode a)
 
 def Forall (tp: TracedProgram f) (P: α → Step α → Memory → Prop): Prop :=
-  ∀ a, foldl tp a (λ b s m ↦ b ∧ P a s m) True = some True
+  ∀ a, foldr tp a True (λ s m b ↦ P a s m ∧ b) = some True
 
-def descends (tp: TracedProgram f) (size: α → ℕ): Prop := tp.Forall
-  (λ | a, .recurse _ _ arg, _ => size arg < size a | _, _, _ => true)
+def descendsOp (size: α → ℕ) (a: α): Step α → Memory → Prop
+| .recurse _ _ arg, _ => size arg < size a
+| _, _ => True
 
-def sound (tp: TracedProgram f): Prop := ∀ a, tp.foldl a (λ v _ _ ↦ v) () = some ()
+def descends (tp: TracedProgram f): (α → ℕ) → Prop := tp.Forall ∘ descendsOp
 
--- theorem fold_sound (tp: TracedProgram f) (a: α) (g: θ → TracedProgram f → Memory → θ) (v: θ) (h: tp.sound):
---     Option.isSome (tp.foldl a g v) := by
---   unfold foldl
+def argsMatchOp (_: α): Step α → Memory → Prop
+| @Step.subroutine _ _ _ src _ _ _ _ _ _ arg, m => Complexity.encode arg = m.getms src
+| .recurse _ src arg, m => Complexity.encode arg = m.getms src
+| _, _ => True
 
+def argsMatch (tp: TracedProgram f): Prop := tp.Forall argsMatchOp
 
+def resultOp: Step α → Memory → Memory → Memory
+| .exit, m, _ => m
+| _, _, m => m
 
--- def soundInternal: TracedProgram f → (α → ℕ) → Memory → α → ℕ → Prop
--- | .exit, _, m, a, _ => m = Complexity.encode (f a)
--- | .op inst next, size, m, a, n => next.soundInternal size (inst.apply m) a n
--- | .branch inst pos neg, size, m, a, n =>
---   match inst.apply m with
---   | true => pos.soundInternal size m a n
---   | false => neg.soundInternal size m a n
--- | .subroutine' dst src _ _ func _ next, size, m, a, n =>
---   ∃ x, some x = Complexity.decode _ (m.getms src) ∧
---     next.soundInternal size (m.setms dst (Complexity.encode (func x))) a n
--- | .recurse dst src next, size, m, a, n =>
---   ∃ x, some x = Complexity.decode _ (m.getms src) ∧
---     next.soundInternal size (m.setms dst (Complexity.encode (f x))) a n
+@[simp] def result (tp: TracedProgram f) (a: α): Option Memory := tp.foldr a 0 resultOp
 
--- def sound (tp: TracedProgram f) (size: α → ℕ): Prop := ∀ a, tp.soundInternal size (Complexity.encode a) a (size a)
+def resultMatches (tp: TracedProgram f): Prop := ∀ a, tp.result a = some (Complexity.encode (f a))
 
+def sound (tp: TracedProgram f) (size: α → ℕ): Prop := ∀ a,
+  foldr tp a True (λ s m b ↦ argsMatchOp a s m ∧ b) = some True ∧
+  foldr tp a True (λ s m b ↦ descendsOp size a s m ∧ b) = some True ∧
+  tp.result a = some (Complexity.encode (f a))
 
+@[simp] theorem argsMatches_op:
+    (foldrInternal (.op (f := f) inst next) m True (λ s m b ↦ argsMatchOp a s m ∧ b) = some True) =
+    (foldrInternal next (inst.apply m) True (λ s m b ↦ argsMatchOp a s m ∧ b) = some True) :=
+  iff_iff_eq.mp ⟨
+    λ h ↦ (Option.map_eq_some'.mp h).elim λ _ h ↦
+      h.left.trans (congrArg _ (eq_true (of_eq_true h.right).right)),
+    λ h ↦ Option.map_eq_some'.mpr ⟨_, h, true_and True⟩ ⟩
 
+@[simp] theorem argsMatches_descend:
+    (foldrInternal (.op (f := f) inst next) m True (λ s m b ↦ descendsOp size a s m ∧ b) = some True) =
+    (foldrInternal next (inst.apply m) True (λ s m b ↦ descendsOp size a s m ∧ b) = some True) :=
+  iff_iff_eq.mp ⟨
+    λ h ↦ (Option.map_eq_some'.mp h).elim λ _ h ↦
+      h.left.trans (congrArg _ (eq_true (of_eq_true h.right).right)),
+    λ h ↦ Option.map_eq_some'.mpr ⟨_, h, true_and True⟩ ⟩
+
+@[simp] theorem resultMatches_descend:
+    (foldrInternal (.op (f := f) inst next) m 0 (λ s m b ↦ resultOp s m b) = some res) =
+    (foldrInternal next (inst.apply m) 0 (λ s m b ↦ resultOp s m b) = some res) :=
+  iff_iff_eq.mp ⟨
+    λ h ↦ (Option.map_eq_some'.mp h).elim λ _ h ↦
+      h.left.trans (congrArg _ h.right),
+    λ h ↦ Option.map_eq_some'.mpr ⟨_, h, rfl⟩ ⟩
+
+@[simp] theorem argsMatches_exit:
+    foldrInternal (.exit (f := f)) m True (λ s m b ↦ argsMatchOp a s m ∧ b) = some True :=
+  congrArg some (true_and True)
+
+@[simp] theorem descendsOp_exit:
+    foldrInternal (.exit (f := f)) m True (λ s m b ↦ descendsOp size a s m ∧ b) = some True :=
+  congrArg some (true_and True)
+
+@[simp] theorem resultMatches_exit:
+    (foldrInternal (.exit (f := f)) m 0 (λ s m b ↦ resultOp s m b) = some res) =
+    (m = res) := iff_iff_eq.mp ⟨ Option.some.inj, congrArg _ ⟩
+
+theorem matchesThunkResultBelow
+    {size: α → ℕ}
+    {a: α}
+    {tp: TracedProgram f}:
+    {current: TracedProgram f} →
+    {m: Memory} →
+    (hs: current.foldrInternal m True (λ s m b ↦ argsMatchOp a s m ∧ b) = some True) →
+    (hd: current.foldrInternal m True (λ s m b ↦ descendsOp size a s m ∧ b) = some True) →
+    (hr: current.foldrInternal m 0 resultOp = some (Complexity.encode (f a))) →
+    (ih: ∀ arg, size arg < size a →
+      tp.toProgram.hasResult (Complexity.encode arg) (Complexity.encode (f arg))) →
+    Stack.hasResult (.execution ⟨m, current.toProgram, tp.toProgram⟩ []) (Complexity.encode (f a))
+| .exit, _, _, _, hr, _ => ⟨1, congrArg Stack.result (Option.some.inj hr)⟩
+| .op _ _, _, hs, hd, hr, ih => Stack.hasResult_of_step (matchesThunkResultBelow
+    ((Option.map_eq_some'.mp hs).elim λ _ h ↦ h.left.trans (congrArg _ (eq_true (of_eq_true h.right).right)))
+    ((Option.map_eq_some'.mp hd).elim λ _ h ↦ h.left.trans (congrArg _ (eq_true (of_eq_true h.right).right)))
+    ((Option.map_eq_some'.mp hr).elim λ _ h ↦ h.left.trans (congrArg _ h.right))
+    ih)
+| .branch inst _ _, m, hs, hd, hr, ih =>
+  dite (inst.apply m)
+    (λ hb ↦ (eq_iff_iff.mp (congrFun (Stack.hasResult_branch_pos hb) _)).mpr
+        (matchesThunkResultBelow
+          ((Option.map_eq_some'.mp ((if_pos hb).symm.trans hs)).elim λ _ h ↦ h.left.trans (congrArg _ (eq_true (of_eq_true h.right).right)))
+          ((Option.map_eq_some'.mp ((if_pos hb).symm.trans hd)).elim λ _ h ↦ h.left.trans (congrArg _ (eq_true (of_eq_true h.right).right)))
+          ((Option.map_eq_some'.mp ((if_pos hb).symm.trans hr)).elim λ _ h ↦ h.left.trans (congrArg _ h.right))
+          ih))
+    (λ hb ↦ (eq_iff_iff.mp (congrFun (Stack.hasResult_branch_neg (Bool.eq_false_of_not_eq_true hb)) _)).mpr
+        (matchesThunkResultBelow
+          ((Option.map_eq_some'.mp ((if_neg hb).symm.trans hs)).elim λ _ h ↦ h.left.trans (congrArg _ (eq_true (of_eq_true h.right).right)))
+          ((Option.map_eq_some'.mp ((if_neg hb).symm.trans hd)).elim λ _ h ↦ h.left.trans (congrArg _ (eq_true (of_eq_true h.right).right)))
+          ((Option.map_eq_some'.mp ((if_neg hb).symm.trans hr)).elim λ _ h ↦ h.left.trans (congrArg _ h.right))
+          ih))
+| subroutine' _ _ _ _ _ comp _, _, hs, hd, hr, ih =>
+    (Option.bind_eq_some'.mp hs).elim λ _ harg ↦
+    (Option.map_eq_some'.mp harg.right).elim λ _ hs ↦
+    Stack.hasResult_subroutine
+      ((of_eq_true hs.right).left ▸ comp.has_result _)
+      (matchesThunkResultBelow
+        (hs.left.trans (congrArg _ (eq_true (of_eq_true hs.right).right)))
+        ((Option.map_eq_some'.mp ((congrArg₂ Option.bind harg.left.symm rfl).trans hd)).elim λ _ h ↦ h.left.trans (congrArg _ (eq_true (of_eq_true h.right).right)))
+        ((Option.map_eq_some'.mp ((congrArg₂ Option.bind harg.left.symm rfl).trans hr)).elim λ _ h ↦ h.left.trans (congrArg _ h.right))
+      ih)
+| .recurse _ _ _, _, hs, hd, hr, ih =>
+    (Option.bind_eq_some'.mp hs).elim λ _ harg ↦
+    (Option.map_eq_some'.mp harg.right).elim λ _ hs ↦
+    (Option.map_eq_some'.mp ((congrArg₂ Option.bind harg.left.symm rfl).trans hd)).elim λ _ hd ↦ (Stack.hasResult_recurse
+      ((of_eq_true hs.right).left ▸ ih _ (of_eq_true hd.right).left)
+      (matchesThunkResultBelow
+        (hs.left.trans (congrArg _ (eq_true (of_eq_true hs.right).right)))
+        (hd.left.trans (congrArg _ (eq_true (of_eq_true hd.right).right)))
+        ((Option.map_eq_some'.mp ((congrArg₂ Option.bind harg.left.symm rfl).trans hr)).elim λ _ h ↦ h.left.trans (congrArg _ h.right))
+        ih))
+
+theorem hasResult (tp: TracedProgram f) {size: α → ℕ} (hs: tp.argsMatch) (hd: tp.descends size) (hr: tp.resultMatches) (n: ℕ):
+    ∀ a, n = size a → tp.toProgram.hasResult (Complexity.encode a) (Complexity.encode (f a)) :=
+  n.strong_induction_on λ _ ih _ ha ↦
+    matchesThunkResultBelow (hs _) (hd _) (hr _)
+      (λ _ hlt ↦ ih _ (ha ▸ hlt) _ rfl)
+
+class HasTrace (f: α → β) where
+  program: List (TracedProgram f → TracedProgram f)
+  size: α → ℕ
+  sound: (build program).sound size
+
+instance [tr: HasTrace f]: Computable Encoding.Model f where
+  program := (build tr.program).toProgram
+  has_result _ := hasResult _ (λ _ ↦ (tr.sound _).left) (λ _ ↦ (tr.sound _).right.left) (λ _ ↦ (tr.sound _).right.right) _ _ rfl
 
 end TracedProgram
-
 end Complexity
 end HMem
