HMem.lean
@@ -4,3 +4,4 @@ import HMem.Encoding.Basic
 import HMem.Encoding.Emulator
 import HMem.Computability.Basic
 import HMem.Computability.Memory
+import HMem.Computability.TracedProgram
